src/coqutil/CoqUtil.v
@@ -382,3 +382,26 @@ Lemma of_tup3_inj {A B C: Type} (x1 x2: ocaml_tup3 A B C):
 Proof.
   auto.
 Qed.
+
+Fixpoint rev_map_aux {A B: Type} (f: A -> B) accu l:=
+  match l with
+  | [] => accu
+  | a :: l => rev_map_aux f (f a :: accu) l
+  end.
+
+Definition rev_map {A B: Type} (f: A -> B) (l: list A) : list B :=
+  rev_map_aux f nil l.
+
+Lemma rev_map_aux_eq {C D: Type} (f: C -> D) accu (l: list C):
+  rev_map_aux f accu l = (map f (rev l)) ++ accu.
+Proof.
+  revert accu.
+  induction l as [| h t IH]; simpl; auto; intros accu.
+  rewrite IH, map_app. simpl. rewrite <- app_assoc. reflexivity.
+Qed.
+
+Lemma rev_map_eq {C D: Type} (f: C -> D) (l: list C):
+  rev_map f l = map f (rev l).
+Proof.
+  unfold rev_map. rewrite rev_map_aux_eq, app_nil_r. reflexivity.
+Qed.
